theory/Z_Scraps.thy
@@ -1,6 +1,100 @@
 theory Z_Scraps
 begin
 
+
+(*
+inductive subexp :: "exp \<Rightarrow> exp \<Rightarrow> bool" ("_ \<preceq>\<^sub>e _" [56,56]55) where
+  Refl : "
+    e \<preceq>\<^sub>e e
+  " | 
+  Let: "
+    \<lbrakk>
+      e \<preceq>\<^sub>e e\<^sub>n
+    \<rbrakk> \<Longrightarrow>
+    e \<preceq>\<^sub>e (LET x = b in e\<^sub>n)
+  " | 
+  Let_Spawn_Child: "
+    \<lbrakk>
+      e \<preceq>\<^sub>e e\<^sub>c
+    \<rbrakk> \<Longrightarrow>
+    e \<preceq>\<^sub>e (LET x = SPAWN e\<^sub>c in e\<^sub>n)
+  " |
+  Let_Case_Left: "
+    \<lbrakk>
+      e \<preceq>\<^sub>e e\<^sub>l
+    \<rbrakk> \<Longrightarrow>
+    e \<preceq>\<^sub>e (LET x = CASE x\<^sub>s LEFT x\<^sub>l |> e\<^sub>l RIGHT x\<^sub>r |> e\<^sub>r in e\<^sub>n)
+  " | 
+  Let_Case_Right: "
+    \<lbrakk>
+      e \<preceq>\<^sub>e e\<^sub>r
+    \<rbrakk> \<Longrightarrow>
+    e \<preceq>\<^sub>e (LET x = CASE x\<^sub>s LEFT x\<^sub>l |> e\<^sub>l RIGHT x\<^sub>r |> e\<^sub>r in e\<^sub>n)
+  " |
+  Let_Abs_Body: "
+    \<lbrakk>
+      e \<preceq>\<^sub>e e\<^sub>b 
+    \<rbrakk> \<Longrightarrow>
+    e \<preceq>\<^sub>e (LET x = FN f x\<^sub>p . e\<^sub>b in e\<^sub>n)
+  "
+
+lemma subexp_trans: "
+  e\<^sub>x \<preceq>\<^sub>e e\<^sub>y \<Longrightarrow> e\<^sub>y \<preceq>\<^sub>e e\<^sub>z \<Longrightarrow> e\<^sub>x \<preceq>\<^sub>e e\<^sub>z
+"
+proof -
+  assume "e\<^sub>x \<preceq>\<^sub>e e\<^sub>y"
+  assume "e\<^sub>y \<preceq>\<^sub>e e\<^sub>z" then
+  have "(\<forall> e\<^sub>x . e\<^sub>x \<preceq>\<^sub>e e\<^sub>y \<longrightarrow> e\<^sub>x \<preceq>\<^sub>e e\<^sub>z)"
+  proof (induction rule: subexp.induct)
+    case (Refl e)
+    show "\<forall>e\<^sub>x. e\<^sub>x \<preceq>\<^sub>e e \<longrightarrow> e\<^sub>x \<preceq>\<^sub>e e" by simp
+  next
+    case (Let e e\<^sub>n x b)
+    assume "e \<preceq>\<^sub>e e\<^sub>n" "\<forall>e\<^sub>x. e\<^sub>x \<preceq>\<^sub>e e \<longrightarrow> e\<^sub>x \<preceq>\<^sub>e e\<^sub>n"
+
+    have "\<forall>e\<^sub>x. e\<^sub>x \<preceq>\<^sub>e e\<^sub>n \<longrightarrow> e\<^sub>x \<preceq>\<^sub>e LET x = b in e\<^sub>n" by (simp add: subexp.Let) 
+    with `\<forall>e\<^sub>x. e\<^sub>x \<preceq>\<^sub>e e \<longrightarrow> e\<^sub>x \<preceq>\<^sub>e e\<^sub>n`
+    show "\<forall>e\<^sub>x. e\<^sub>x \<preceq>\<^sub>e e \<longrightarrow> e\<^sub>x \<preceq>\<^sub>e LET x = b in e\<^sub>n" by blast
+  next
+    case (Let_Spawn_Child e e\<^sub>c x e\<^sub>n)
+    assume "e \<preceq>\<^sub>e e\<^sub>c" "\<forall>e\<^sub>x. e\<^sub>x \<preceq>\<^sub>e e \<longrightarrow> e\<^sub>x \<preceq>\<^sub>e e\<^sub>c"
+
+    have "\<forall>e\<^sub>x. e\<^sub>x \<preceq>\<^sub>e e\<^sub>c \<longrightarrow> e\<^sub>x \<preceq>\<^sub>e LET x = SPAWN e\<^sub>c in e\<^sub>n" by (simp add: subexp.Let_Spawn_Child)
+    with `\<forall>e\<^sub>x. e\<^sub>x \<preceq>\<^sub>e e \<longrightarrow> e\<^sub>x \<preceq>\<^sub>e e\<^sub>c`
+    show "\<forall>e\<^sub>x. e\<^sub>x \<preceq>\<^sub>e e \<longrightarrow> e\<^sub>x \<preceq>\<^sub>e LET x = SPAWN e\<^sub>c in e\<^sub>n"by blast
+  next
+    case (Let_Case_Left e e\<^sub>l x x\<^sub>s x\<^sub>l x\<^sub>r e\<^sub>r e\<^sub>n)
+    assume "e \<preceq>\<^sub>e e\<^sub>l" "\<forall>e\<^sub>x. e\<^sub>x \<preceq>\<^sub>e e \<longrightarrow> e\<^sub>x \<preceq>\<^sub>e e\<^sub>l"
+
+    have "\<forall>e\<^sub>x. e\<^sub>x \<preceq>\<^sub>e e\<^sub>l \<longrightarrow> e\<^sub>x \<preceq>\<^sub>e LET x = CASE x\<^sub>s LEFT x\<^sub>l |> e\<^sub>l RIGHT x\<^sub>r |> e\<^sub>r in e\<^sub>n" by (simp add: subexp.Let_Case_Left)
+    with `\<forall>e\<^sub>x. e\<^sub>x \<preceq>\<^sub>e e \<longrightarrow> e\<^sub>x \<preceq>\<^sub>e e\<^sub>l`
+    show "\<forall>e\<^sub>x. e\<^sub>x \<preceq>\<^sub>e e \<longrightarrow> e\<^sub>x \<preceq>\<^sub>e LET x = CASE x\<^sub>s LEFT x\<^sub>l |> e\<^sub>l RIGHT x\<^sub>r |> e\<^sub>r in e\<^sub>n" by blast
+  next
+    case (Let_Case_Right e e\<^sub>r x x\<^sub>s x\<^sub>l e\<^sub>l x\<^sub>r e\<^sub>n)
+    assume "e \<preceq>\<^sub>e e\<^sub>r" "\<forall>e\<^sub>x. e\<^sub>x \<preceq>\<^sub>e e \<longrightarrow> e\<^sub>x \<preceq>\<^sub>e e\<^sub>r"
+
+    have "\<forall>e\<^sub>x. e\<^sub>x \<preceq>\<^sub>e e\<^sub>r \<longrightarrow> e\<^sub>x \<preceq>\<^sub>e LET x = CASE x\<^sub>s LEFT x\<^sub>l |> e\<^sub>l RIGHT x\<^sub>r |> e\<^sub>r in e\<^sub>n" by (simp add: subexp.Let_Case_Right)
+    with `\<forall>e\<^sub>x. e\<^sub>x \<preceq>\<^sub>e e \<longrightarrow> e\<^sub>x \<preceq>\<^sub>e e\<^sub>r`
+    show "\<forall>e\<^sub>x. e\<^sub>x \<preceq>\<^sub>e e \<longrightarrow> e\<^sub>x \<preceq>\<^sub>e LET x = CASE x\<^sub>s LEFT x\<^sub>l |> e\<^sub>l RIGHT x\<^sub>r |> e\<^sub>r in e\<^sub>n" by blast
+  next
+    case (Let_Abs_Body e e\<^sub>b x f x\<^sub>p e\<^sub>n)
+    assume "e \<preceq>\<^sub>e e\<^sub>b" "\<forall>e\<^sub>x. e\<^sub>x \<preceq>\<^sub>e e \<longrightarrow> e\<^sub>x \<preceq>\<^sub>e e\<^sub>b"
+
+    have "\<forall>e\<^sub>x. e\<^sub>x \<preceq>\<^sub>e e\<^sub>b \<longrightarrow> e\<^sub>x \<preceq>\<^sub>e LET x = FN f x\<^sub>p . e\<^sub>b in e\<^sub>n" by (simp add: subexp.Let_Abs_Body)
+    with `\<forall>e\<^sub>x. e\<^sub>x \<preceq>\<^sub>e e \<longrightarrow> e\<^sub>x \<preceq>\<^sub>e e\<^sub>b`
+    show "\<forall>e\<^sub>x. e\<^sub>x \<preceq>\<^sub>e e \<longrightarrow> e\<^sub>x \<preceq>\<^sub>e LET x = FN f x\<^sub>p . e\<^sub>b in e\<^sub>n" by blast
+  qed 
+  with `e\<^sub>x \<preceq>\<^sub>e e\<^sub>y`
+  show "e\<^sub>x \<preceq>\<^sub>e e\<^sub>z" by blast
+qed
+
+lemma subexp1: "
+  e\<^sub>n \<preceq>\<^sub>e LET x = b in e\<^sub>n
+"
+by (simp add: Let Refl)
+
+*)
+
 (*
 
 type_synonym flow_set = "(exp \<times> control_label \<times> exp) set"
